Proved correctness of prop_exec_preserves_well_formed checker
... under some strong (but natural) assumptions about genState

In the meanwhile run into some very silly unification problem,
that Zoe previously hacked around by adding overlapping type
class instances. The main problem is that Coq can't figure out
"Testable (Property Gen)" although it knows "Testable (Gen QPred)"
and Property is defined as follows:
Definition Property (Gen: Type -> Type) : Type := Gen QProp.
Ended up adding lots of silly type annotations to work around
Coq's silliness.

ifc/extended/Testing/SanityChecks.v
@@ -14,12 +14,12 @@ Require Import List.
 Require Import Common.
 Require Import String.
 
+Require Import ssreflect ssrbool eqtype.
+
 Local Open Scope string.
+
 (* Sanity check for stamp generation *)
-
-Definition Property := Property Gen.Gen. 
-
-Definition prop_stamp_generation (st : State) :=
+Definition prop_stamp_generation (st : State) : Property Gen.Gen :=
   whenFail (show st) (well_formed st).
 
 (*
@@ -30,26 +30,58 @@ Definition propStampGeneration (st : State) :=
            (wellFormed st stamps).
 *)
 
-Definition prop_exec_preserves_well_formed (t : table) 
-: Property :=
-  forAllShrink show arbitrary (fun _ => []) (fun st =>
-  if well_formed st then
-    match exec t st with
-    | Some (_, st') =>
-      whenFail ("Initial: " ++ show st ++ nl ++
-                "Step to: " ++ show st' ++ nl)
-               (well_formed st')
-    | _ => property rejected
-    end
-  else property false).
-
-Definition exec_preserves_well_formed : Prop := forall t st x st',
-  well_formed st = true ->
-  exec t st = Some (x, st') ->
-  well_formed st' = true.
-
-Definition prop_generate_indist
-: Property :=
+Definition prop_generate_indist : Property Gen.Gen :=
   forAllShrink show gen_variation_state (fun _ => []) (* shrinkVState *)
                (fun v => let '(Var lab st1 st2) := v in
-                property (indist lab st1 st2)).
+                property (indist lab st1 st2) : Gen.Gen QProp).
+
+Section Checkers.
+  Context {Gen : Type -> Type}
+          {H : GenMonad Gen}.
+  
+  Definition prop_exec_preserves_well_formed (t : table) 
+  : Property Gen :=
+    forAllShrink show arbitrary (fun _ => []) (fun st =>
+    (if well_formed st then
+      match exec t st with
+      | Some (_, st') =>
+        whenFail ("Initial: " ++ show st ++ nl ++
+                  "Step to: " ++ show st' ++ nl)
+                 (well_formed st')
+      | _ => property rejected
+      end
+    else property false) : Gen QProp).
+
+End Checkers.
+
+Definition exec_preserves_well_formed t : Prop := forall st x st',
+  well_formed st ->
+  exec t st = Some (x, st') ->
+  well_formed st'.
+
+Require Import EndToEnd SetOfOutcomes.
+
+(* One direction of this (soundness) checked by prop_stamp_generation above;
+   this is the high-level spec we need for genState *)
+Lemma genState_well_formed : forall st,
+  @genState Pred _ st <-> well_formed st.
+Admitted.
+
+Lemma prop_exec_preserves_well_formed_equiv:
+  forall (t : table), 
+    semProperty (@prop_exec_preserves_well_formed Pred _ t) <->
+    exec_preserves_well_formed t.
+Proof.
+  move => t.
+  rewrite /prop_exec_preserves_well_formed /exec_preserves_well_formed
+    semForAllShrink /arbitrary /arbState. setoid_rewrite semPredQProp.
+  split => [H st tr st' wf ex | H st arb].
+  - assert (@genState Pred _ st) as gs by (by rewrite genState_well_formed).
+    specialize (H st gs).
+    rewrite wf ex in H. by move /semWhenFail_idemp /semBool in H.
+  - move /genState_well_formed in arb. rewrite arb. specialize (H st).
+    move : H. case (exec t st) => [ [tr st'] | ] H.
+    + specialize (H tr st' arb Logic.eq_refl). rewrite H.
+      rewrite semWhenFail_idemp. by rewrite <- semBool.   
+    + fold (semTestable rejected). rewrite <- semResult. reflexivity.
+Qed.
