ifc/extended/Testing/SSNI.v
@@ -23,13 +23,14 @@ Section Checkers.
   Context {Gen : Type -> Type}
           {H : GenMonad Gen}.
   
-  Definition Property := Property Gen.
+(*  Definition Property := Property Gen. *)
 
 
   Definition is_low_state st lab := isLow (pc_lab (st_pc st)) lab.
 
+Set Printing All.
 
-  Definition propSSNI_helper (t : table) (v : Variation) : Property :=
+  Definition propSSNI_helper (t : table) (v : Variation) : Property Gen :=
     let '(Var lab st1 st2) := v in
     (*  Property.trace (Show.show lab ++ Show.nl ++
      showStatePair lab frameMap1 frameMap2 st1 st2) *)   
@@ -40,19 +41,19 @@ Section Checkers.
             (if indist lab st1 st2 then
                (* XXX Our generator should always give us this by design.
                   If that's not the case the generator is broken. *)
-               match exec t st1 return Property with
+               match exec t st1 return Gen QProp with
                  | Some (tr1, st1') =>
                    if is_low_state st1 lab then
                      match exec t st2 with
                        | Some (tr2, st2') =>
                          collect "LOW -> *" (
-                                   whenFail 
+                                   whenFail
                                      ("LOW -> *" ++ nl ++
                                                  (show_execution lab [st1; st1'] [st2; st2']))
                                      (observe_comp (observe lab tr1) (observe lab tr2) 
-                                                   && (indist lab st1' st2')))
+                                                   && (indist lab st1' st2')):Gen QProp)
                        | _ => (* 1 took a low step and 2 failed *)
-                         collect "Second failed" (property true)
+                         collect "Second failed" (property true : Gen QProp)
                      (* 
                 ((Property.trace (show_pair lab st1 st1'))
                 (property false))
@@ -66,15 +67,15 @@ Section Checkers.
                          | Some (tr2, st2') =>
                            if is_low_state st2' lab then 
                              collect "HIGH -> LOW" (
-                                       (whenFail ("HIGH -> LOW" ++ Show.nl ++
+                                       whenFail ("HIGH -> LOW" ++ Show.nl ++
                                                                 (show_execution lab [st1; st1'] [st2; st2']))
                                                  (observe_comp (observe lab tr1) (observe lab tr2) 
-                                                               && (indist lab st1' st2')))
+                                                               && (indist lab st1' st2')) : Gen QProp
                                      )
-                           else collect "Second not low" (property true)
+                           else collect "Second not low" (property true : Gen QProp)
                          (* This can happen; it's just a discard *)
                          (* TODO: could check that st2' `indist` st1 *)
-                         | _ => collect "Second failed H" (property true)
+                         | _ => collect "Second failed H" (property true : Gen QProp)
                        (* This can happen; it's just a discard *)
                        end
                      else
@@ -83,17 +84,19 @@ Section Checkers.
                                                           (show_pair lab st1 st1'))
                                           (beq_nat (List.length (observe lab tr1)) 0 
                                        && indist lab st1 st1')
-                               )
-                 | _ => collect "Failed" (property true)
+                               : Gen QProp)
+                 | _ => collect "Failed" (property true : Gen QProp)
                (* This can happen; it's just a discard *)
                (* TODO: could check if st2 does a H -> H step *)
                end
-             else collect "Not indist!" (property true)).
+             else collect "Not indist!" (property true : Gen QProp)).
            (* XXX this should never happen with a correct generator;
               and prop_generate_indist already tests this;
               so this should either go away or become (propery false) *)
 
-  Definition propSSNI t : Property := 
-    forAllShrink (fun _ => ""%string) gen_variation_state (fun _ => nil) (* shrinkVState *) (propSSNI_helper t).
+  Definition propSSNI t : Property Gen := 
+    forAllShrink (fun _ => ""%string) gen_variation_state (fun _ => nil)
+      (* shrinkVState *)
+      (propSSNI_helper t : @Variation Machine.State -> Gen QProp).
 
 End Checkers.
